- moved trans syst from KVS to ET theory - checkpoint, requires substantial cleanup

txn-data-consistency/Execution_Tests.thy
@@ -4,6 +4,247 @@ theory Execution_Tests
   imports Key_Value_Stores
 begin
 
+subsection \<open>Execution Tests as Transition Systems\<close>
+
+definition visTx :: "('v, 'm) kvs_store \<Rightarrow> view \<Rightarrow> txid set" where
+  "visTx K u \<equiv> {v_writer (K k!i) | i k. i \<in> u k}"
+
+definition read_only_Txs :: "('v, 'm) kvs_store \<Rightarrow> txid set" where
+  "read_only_Txs K \<equiv> Tn ` kvs_readers K - kvs_writers K"
+
+lemma visTx_subset_kvs_writers: "view_in_range K u \<Longrightarrow> visTx K u \<subseteq> kvs_writers K"
+  apply (auto simp add: visTx_def kvs_writers_def vl_writers_def)
+  subgoal for i k by (auto intro: exI[where x=k])
+  done
+
+lemma union_write_read_only [simp]: "kvs_writers K \<union> read_only_Txs K = kvs_txids K"
+  by (simp add: read_only_Txs_def kvs_txids_def)
+
+lemma inter_write_read_only [simp]: "kvs_writers K \<inter> read_only_Txs K = {}"
+  by (simp add: read_only_Txs_def Diff_triv)
+
+lemma inter_visTx_read_only [simp]: "view_in_range K u \<Longrightarrow> visTx K u \<inter> read_only_Txs K = {}"
+  using visTx_subset_kvs_writers inter_write_read_only by blast
+
+
+text \<open>Closedness: Here is the original definition from the ECOOP paper.\<close>
+
+abbreviation closed_orig :: "('v, 'm) kvs_store \<Rightarrow> view \<Rightarrow> txid rel \<Rightarrow> bool" where
+  "closed_orig K u r \<equiv> closed_general' (visTx K u) (r^-1) (read_only_Txs K)"
+
+lemma closed_orig_is_orig_indeed:
+  "closed_orig K u r \<longleftrightarrow> visTx K u = (((r\<^sup>*)^-1) `` (visTx K u)) - (read_only_Txs K)"
+  by (simp add: closed_general'_def rtrancl_converse)
+
+
+text \<open>Closedness, modified definition: @{term "visTx K u"} closed under @{term "(r^-1)\<^sup>+"}} up to
+@{term "read_only_Txs K"}.\<close>
+
+abbreviation closed :: "('v, 'm) kvs_store \<Rightarrow> view \<Rightarrow> txid rel \<Rightarrow> bool" where
+  "closed K u r \<equiv> closed_general (visTx K u) (r^-1) (read_only_Txs K)"
+
+lemma closed_equiv_closed_orig: 
+  shows "view_in_range K u \<Longrightarrow> closed K u r \<longleftrightarrow> closed_orig K u r"
+  by (simp add: closed_general_equiv)
+
+
+subsection \<open>Execution Tests\<close>
+
+datatype 'v label = ET cl_id sqn view "'v fingerpr" | ETSkip
+
+locale ExecutionTest =
+  fixes R_ET :: "'v kv_store \<Rightarrow> 'v fingerpr \<Rightarrow> txid rel"
+    and vShift :: "'v kv_store \<Rightarrow> view \<Rightarrow> 'v kv_store \<Rightarrow> view \<Rightarrow> bool"
+   \<comment>\<open>We need some assumptions from Definition 8 of ECOOP paper\<close>
+begin
+
+definition canCommit :: "'v kv_store \<Rightarrow> view \<Rightarrow> 'v fingerpr \<Rightarrow> bool" where
+  "canCommit K u F \<equiv> closed K u (R_ET K F)"
+
+fun ET_cl_txn :: "cl_id \<Rightarrow> sqn \<Rightarrow> view \<Rightarrow> 'v fingerpr \<Rightarrow> ('v kv_store \<times> view) \<Rightarrow> ('v kv_store \<times> view) \<Rightarrow> bool" where
+  "ET_cl_txn cl sn u'' F (K, u) (K', u') \<longleftrightarrow> (\<exists>t.
+    view_wellformed K u'' \<and>
+    view_wellformed K' u' \<and>
+    canCommit K u'' F \<and> vShift K u'' K' u' \<and> \<comment>\<open>From here is not in Execution Test of the thesis\<close>
+    u \<sqsubseteq> u'' \<and>
+    view_wellformed K u \<and>       \<comment> \<open>chsp: do we need this one?\<close>
+    t = Tn_cl sn cl \<and>
+    t \<in> next_txids K cl \<and>
+    K' = update_kv t F u'' K)"
+
+declare ET_cl_txn.simps [simp del]
+lemmas ET_cl_txn_def = ET_cl_txn.simps
+
+fun ET_trans_and_fp :: "'v config \<Rightarrow> 'v label \<Rightarrow> 'v config \<Rightarrow> bool" where
+  "ET_trans_and_fp (K , U) (ET cl sn u'' F) (K', U') \<longleftrightarrow>
+    (\<exists>u'. ET_cl_txn cl sn u'' F (K, U cl) (K', u') \<and> U' = U (cl := u')) \<and> fp_property F K u''" |
+  "ET_trans_and_fp c ETSkip c' \<longleftrightarrow> c' = c"
+
+lemmas ET_trans_induct = ET_trans_and_fp.induct [case_names ET_txn]
+
+definition ET_ES :: "('v label, 'v config) ES" where
+  "ET_ES \<equiv> \<lparr>
+    init = (=) config_init,
+    trans = ET_trans_and_fp
+  \<rparr>"
+
+lemmas ET_init_def = config_init_defs
+lemmas ET_trans_def = ET_cl_txn_def
+lemmas ET_ES_defs = ET_ES_def ET_init_def
+
+lemma trans_ET_ES_eq [simp]: "(ET_ES: s \<midarrow>e\<rightarrow> s') \<longleftrightarrow> ET_trans_and_fp s e s'"
+  by (auto simp add: ET_ES_def)
+
+
+subsubsection \<open>Proof rule for ET refinement\<close>
+
+text \<open>Simple rule to structure proofs of the ET transition refinement. Note that variable 
+@{term "u'"} does not appear in conclusion and should be instantiated appropriately.}\<close>
+
+lemma ET_trans_rule:
+  assumes 
+    \<open>U cl \<sqsubseteq> u''\<close>
+    \<open>canCommit K u'' F\<close>
+    \<open>vShift K u'' K' u'\<close>
+    \<open>view_wellformed K u''\<close> 
+    \<open>view_wellformed K' u'\<close>
+    \<open>view_wellformed K (U cl)\<close>      
+    \<open>Tn_cl sn cl \<in> next_txids K cl\<close>
+    \<open>fp_property F K u''\<close>
+    \<open>K' = update_kv (Tn_cl sn cl) F u'' K\<close>
+    \<open>U' = U(cl := u')\<close>
+  shows \<open>ET_trans_and_fp (K , U) (ET cl sn u'' F) (K', U')\<close>
+  using assms
+  by (auto simp add: ET_cl_txn_def)
+
+
+subsubsection \<open>Wellformedness Invariants\<close>
+
+\<comment> \<open>Invariant\<close>
+
+lemma reach_snapshot_property [simp, dest]:
+  assumes "reach ET_ES s"
+  shows "snapshot_property (fst s)" \<comment> \<open>fst s: kvs part of state\<close>
+  using assms
+proof(induction s rule: reach.induct)
+  case (reach_init s)
+  then show ?case
+    by (auto simp add: ET_ES_defs)
+next
+  case (reach_trans s e s')
+  then show ?case 
+  proof (induction s e s' rule: ET_trans_induct)
+    case (ET_txn K U cl sn u'' F K' U')
+    then show ?case
+      apply (auto simp add: ET_trans_def intro!: kvs_wellformed_intros)
+      subgoal for k i j u' x \<comment> \<open>subgoal for the readerset case\<close>
+        apply (cases "i \<in> full_view (K k)"; cases "j \<in> full_view (K k)";
+               auto dest!: not_full_view_update_kv update_kv_new_version_v_readerset)
+        by (cases "i = Max (u'' k)"; cases "j = Max (u'' k)";
+               auto simp add: snapshot_property_def v_readerset_update_kv_rest_inv
+               fresh_txid_v_reader_set dest!: v_readerset_update_kv_max_u )
+      subgoal for k i j u'  \<comment> \<open>subgoal for the writer case\<close>
+        using update_kv_length [of "Tn_cl sn cl" F u'' K k]
+        by (cases "i \<in> full_view (K k)"; cases "j \<in> full_view (K k)";
+            auto simp add: snapshot_property_def less_Suc_eq_le full_view_def update_kv_v_writer_inv
+                 dest!: update_kv_new_version_v_writer fresh_txid_v_writer)
+      done
+  qed simp
+qed
+
+
+lemma reach_wr_so [simp, dest]:
+  assumes "reach ET_ES s"
+  shows "wr_so (fst s)"
+  using assms
+proof(induction s rule: reach.induct)
+  case (reach_init s)
+  then show ?case 
+    by (auto simp add: ET_ES_defs)
+next
+  case (reach_trans s e s')
+  then show ?case 
+  proof (induction s e s' rule: ET_trans_induct)
+    case (ET_txn K U cl sn u'' F K' U')
+    then show ?case 
+      apply (auto simp add: ET_trans_def intro!: kvs_wellformed_intros)
+      subgoal for k i x t apply (cases "i \<in> full_view (K k)")
+        subgoal by (cases "i = Max (u'' k)")
+                   (auto simp add: v_readerset_update_kv_rest_inv update_kv_v_writer_inv
+                         dest!: v_readerset_update_kv_max_u fresh_txid_writer_so)
+        subgoal by (auto simp add: update_kv_new_version_v_readerset dest!: not_full_view_update_kv)
+        done
+      subgoal for k i x t apply (cases "i \<in> full_view (K k)")
+        subgoal apply (auto simp add: wr_so_def)
+          by (metis fresh_txid_v_writer update_kv_v_writer_inv v_readerset_update_kv_max_u
+              v_readerset_update_kv_rest_inv image_eqI view_wellformedD1)
+        subgoal by (auto simp add: update_kv_new_version_v_readerset dest!: not_full_view_update_kv)
+        done
+      done
+  qed simp
+qed
+
+
+lemma reach_ww_so [simp, dest]:
+  assumes "reach ET_ES s"
+  shows "ww_so (fst s)"
+  using assms
+proof(induction s rule: reach.induct)
+  case (reach_init s)
+  then show ?case 
+    by (auto simp add: ET_ES_defs)
+next
+  case (reach_trans s e s')
+  then show ?case 
+  proof (induction s e s' rule: ET_trans_induct)
+    case (ET_txn K U cl sn u'' F K' U')
+    then show ?case 
+      apply (auto simp add: ET_trans_def intro!: kvs_wellformed_intros)
+      subgoal for k i x t apply (cases "x \<in> full_view (K k)")
+        subgoal by (auto simp add: update_kv_v_writer_inv full_view_def)
+        subgoal by (auto simp add: update_kv_new_version_v_writer update_kv_v_writer_inv
+                            dest!: not_full_view_update_kv fresh_txid_writer_so)
+        done
+      subgoal for k i x t apply (cases "x \<in> full_view (K k)")
+        subgoal by (auto simp add: ww_so_def update_kv_v_writer_inv full_view_def)
+        subgoal by (auto simp add: update_kv_new_version_v_writer update_kv_v_writer_inv
+                            dest!: not_full_view_update_kv fresh_txid_v_writer)
+        done
+      done
+  qed simp
+qed
+
+
+lemma reach_kvs_initialized [simp, dest]:
+  assumes "reach ET_ES s"
+  shows "kvs_initialized (fst s)"
+  using assms
+proof(induction s rule: reach.induct)
+  case (reach_init s)
+  then show ?case 
+    by (auto simp add: ET_ES_defs)
+next
+  case (reach_trans s e s')
+  then show ?case 
+  proof (induction s e s' rule: ET_trans_induct)
+    case (ET_txn K U cl sn u'' F K' U')
+    then show ?case
+      apply (auto 4 3 simp add: ET_trans_def update_kv_v_value_inv view_zero_full_view 
+                   intro!: kvs_wellformed_intros)
+      subgoal for k using update_kv_length [of "Tn_cl sn cl" F u'' K k]
+        by (auto simp add: kvs_initialized_def).
+  qed simp
+qed
+
+lemma reach_kvs_wellformed [simp, dest]:
+  assumes "reach ET_ES s"
+  shows "kvs_wellformed (fst s)"
+  using assms
+  by (simp add: kvs_wellformed_def)
+
+end
+
+
 subsection \<open>Dependency Relations\<close>
 
 type_synonym 'v dep_rel = "'v kv_store \<Rightarrow> key \<Rightarrow> txid rel"
@@ -21,6 +262,7 @@ definition RW :: "'v dep_rel" where
 
 definition R_onK :: "'v dep_rel \<Rightarrow> 'v kv_store \<Rightarrow> txid rel" where
   "R_onK r K \<equiv> \<Union>k. r K k"
+
 
 subsection \<open>Consistency models' execution tests\<close>
 
@@ -47,10 +289,36 @@ definition vShift_MR :: "view \<Rightarrow> view \<Rightarrow> bool" where
 
 definition vShift_RYW :: "'v kv_store \<Rightarrow> view \<Rightarrow> 'v kv_store \<Rightarrow> view \<Rightarrow> bool" where
   "vShift_RYW K u K' u' \<equiv>
-    \<forall>t \<in> kvs_txids K' - kvs_txids K. \<forall>k i. (v_writer (K' k!i) , t) \<in> SO^= \<longrightarrow> i \<in> u' k"
+    \<forall>t \<in> kvs_txids K' - kvs_txids K. \<forall>k. \<forall>i < length (K' k). 
+      (v_writer (K' k!i) , t) \<in> SO^= \<longrightarrow> i \<in> u' k"
 
 definition vShift_MR_RYW :: "'v kv_store \<Rightarrow> view \<Rightarrow> 'v kv_store \<Rightarrow> view \<Rightarrow> bool" where
   "vShift_MR_RYW K u K' u' \<equiv> vShift_MR u u' \<and> vShift_RYW K u K' u'"
+
+
+text \<open>Lemmas about session guarantees\<close>
+
+lemma vShift_MR_I: "u \<sqsubseteq> u' \<Longrightarrow> vShift_MR u u'" 
+  by (simp add: vShift_MR_def)
+
+lemma vShift_RYW_I:
+  assumes "\<And>t k i. 
+     \<lbrakk> t \<in> kvs_txids K'; t \<notin> kvs_txids K; i < length (K' k); t = v_writer (K' k ! i) \<rbrakk>
+      \<Longrightarrow> i \<in> u' k"
+  and "\<And>t k i. 
+     \<lbrakk> t \<in> kvs_txids K'; t \<notin> kvs_txids K; i < length (K' k); (v_writer (K' k ! i), t) \<in> SO \<rbrakk>
+      \<Longrightarrow> i \<in> u' k"
+  shows "vShift_RYW K u K' u'"
+  using assms
+  by (auto simp add: vShift_RYW_def)
+
+text \<open>combine the two lemmas above into one\<close>
+
+lemmas vShift_MR_RYW_I = 
+  vShift_MR_RYW_def[THEN meta_eq_to_obj_eq, THEN iffD2, OF conjI, OF vShift_MR_I vShift_RYW_I]
+
+
+subsection \<open>Model Instances\<close>
 
 interpretation ET_MR: ExecutionTest "\<lambda>K F. {}" "\<lambda>K u K' u'. vShift_MR u u'" .
 
